Tests/MysqlDriverT.lean
@@ -23,6 +23,13 @@ def main : IO UInt32 := do
   | some conn =>
   DriverRegressions.checkDoubleQueries (fun q ps => conn.query q ps)
   DriverRegressions.checkCompilerQueries .mysql (fun q => conn.query q) conn.execRaw
+  DriverRegressions.checkAggregateDml .mysql {
+    query := fun q => conn.query q
+    update := fun q => conn.execUpdate q
+    delete := fun q => conn.execDelete q
+    queryAlias := fun q => conn.query q
+    updateAlias := fun q => conn.execUpdate q
+    execRaw := conn.execRaw }
   conn.execRaw (setupSql .mysql)
   let ops : DriverOps := {
     query := fun q => conn.query q seedParams
